jar2bpl_test/regression/false_positives/fp01/FalsePositives01.java
@@ -1,0 +1,81 @@
+import java.util.Enumeration;
+
+
+public class FalsePositives01 {
+
+	private String[] sourceKeys;
+	String[] sourceValues;
+
+	String[] removeKeys;
+	String[] removeValues;
+	
+	private int countSource;
+	
+
+//	public int foo() {return 1;}
+//	public Enumeration bar() {return null;}
+//	
+//	public void removeAttribute()
+//	{
+//		try
+//		{
+//			
+//			boolean hit = false;
+//			for(int countSource = 0; countSource < sourceKeys.length; countSource++)
+//			{
+//				hit = false;
+//				if(sourceKeys[countSource] == "name" )
+//				{
+//					hit = true;
+//				}
+//
+//							
+//				if(!hit)
+//				{
+//					//THIS IS THE IMPORTANT LINE!
+//					sourceKeys[countSource].toString(); 
+//				}
+//			}
+//		}
+//		catch (ClassCastException cce)
+//		{
+//			
+//		}
+//	}
+//	
+	
+//	public void FalsePositive01() {
+//		boolean hit = false;		
+//		int counter = 0;
+//		do
+//		{
+//			hit = false;
+//			if(countSource  > counter)
+//			{
+//				counter++;
+//				hit = true;
+//				if(counter > 10000)
+//				{
+//					return;
+//				}
+//			}
+//		} while(hit);		
+//		countSource = 3; //do something just to have code here.
+//	}
+//
+	public void FalsePositive02(Object htmlTag) {
+		if (htmlTag.toString().compareTo("strike")==0)
+		{
+			countSource=1;
+		}
+		else if (htmlTag.toString().compareTo("sup")==0)
+		{
+			countSource=2;
+		}
+		else if (htmlTag.toString().compareTo("sub")==0)
+		{
+			countSource=3;
+		}		
+	}
+	
+}
