jar2bpl_test/regression/false_positives/fp03/FalsePositives03.java
@@ -1,0 +1,22 @@
+
+
+import java.awt.Container;
+
+import javax.naming.Context;
+
+public class FalsePositives03 {
+
+	/*
+	 * there is an axiom missing that states that  
+	 * null <: X for all X, otherwise the case where
+	 * container==null would inevitably crash the cast.
+	 */
+	public void foo(Container container) {
+        if (container instanceof Context || container == null) {
+            Context ctx = ((Context) container); //not sure
+        } else {
+          //nothing
+        }		
+	}
+	
+}
