jar2bpl_test/src/jar2bpl_test/BouncyCastleTranslationTest.java
@@ -1,0 +1,37 @@
+package jar2bpl_test;
+
+import static org.junit.Assert.fail;
+
+import org.joogie.Dispatcher;
+import org.joogie.Options;
+import org.junit.Test;
+
+public class BouncyCastleTranslationTest {
+
+	
+	@Test
+	public void testJarInputFile() {
+		//TODO: design one test case for each sort of input to the translation.
+		try {
+			String javaFileDir = System.getProperty("user.dir")+"/regression/bc/java";
+			Options.v().setClasspath(javaFileDir);			
+			//Options.v().setSoundThreads(true);
+			String bplFile = "regression/test_output/bc.bpl";
+
+			Dispatcher.run(javaFileDir,
+					bplFile);
+			
+		} catch (Exception e) {			
+			fail("Translation Error " + e.toString());
+		}
+		
+		org.junit.Assert.assertTrue(true);
+	}
+	
+
+	
+	
+}
+
+
+
