jar2bpl_test/src/jar2bpl_test/TestFalsePositives.java
@@ -1,0 +1,78 @@
+package jar2bpl_test;
+/**
+ * 
+ */
+
+
+import static org.junit.Assert.fail;
+
+import java.io.File;
+import java.util.Collection;
+import java.util.LinkedList;
+
+import org.joogie.Dispatcher;
+import org.joogie.Options;
+import org.junit.Test;
+import org.junit.runner.RunWith;
+import org.junit.runners.Parameterized;
+
+/**
+ * @author schaef
+ *
+ */
+@RunWith(Parameterized.class)
+public class TestFalsePositives  {
+	
+	@Parameterized.Parameters (name = "{index}: check ({1})")
+	public static Collection<Object[]> data() {
+		LinkedList<Object[]> filenames = new LinkedList<Object[]>();
+		String dirname = System.getProperty("user.dir")+"/regression/false_positives";
+		  File dir = new File(dirname);
+		  File[] directoryListing = dir.listFiles();
+		  if (directoryListing != null) {
+		    for (File child : directoryListing) {		    	
+		    	if (child.isDirectory() && child.getAbsolutePath()!=null) {
+		    		filenames.add(new Object[] {child.getAbsolutePath()});
+		    		
+		    	} else {
+		    		//Ignore
+		    	}
+		    }
+		  } else {			  
+		    // Handle the case where dir is not really a directory.
+		    // Checking dir.isDirectory() above would not be sufficient
+		    // to avoid race conditions with another process that deletes
+		    // directories.
+			  throw new RuntimeException(dirname + " NOT FOUND!");
+		  }				  
+	   return filenames;
+   }
+	
+    private String input;
+    
+    public TestFalsePositives(String input) {
+        this.input = input;
+    }
+
+	
+	@Test
+	public void test() {
+		System.out.println("Test: "+this.input);
+		try {			
+			String javaFileDir = this.input;
+			Options.v().setClasspath(javaFileDir);
+			String bplFile = "regression/test_output/fic.bpl";
+
+			Dispatcher.run(javaFileDir,
+					bplFile);
+
+			System.err.println("============ PASSED =================");
+		} catch (Exception e) {
+			fail("Translation Error " + e.toString());
+		}
+		
+		org.junit.Assert.assertTrue(true);
+		
+	}
+
+}
