jar2bpl_test/regression/test_output/java_input.bpl
@@ -10,14 +10,12 @@ const unique $null : ref;
 const unique $type : Field javaType;
 const unique $alloc : Field bool;
 const { :sourceloc "Object.java",-1,-1,-1,-1 } unique java.lang.Object : javaType extends  complete;
-const { :sourceloc "FalsePositives.java",-1,-1,-1,-1 } unique FalsePositives : javaType extends  unique java.lang.Object complete;
+const { :sourceloc "InfeasibleCode01.java",-1,-1,-1,-1 } unique InfeasibleCode01 : javaType extends  unique java.lang.Object complete;
 const { :sourceloc "Serializable.java",-1,-1,-1,-1 } unique java.io.Serializable : javaType extends  unique java.lang.Object complete;
 const { :sourceloc "Comparable.java",-1,-1,-1,-1 } unique java.lang.Comparable : javaType extends  unique java.lang.Object complete;
 const { :sourceloc "CharSequence.java",-1,-1,-1,-1 } unique java.lang.CharSequence : javaType extends  unique java.lang.Object complete;
-const { :sourceloc "String.java",-1,-1,-1,-1 } unique java.lang.String : javaType extends  unique java.lang.CharSequence, unique java.lang.Object, unique java.lang.Comparable, unique java.io.Serializable complete;
-const unique $StringConst0 : ref extends  complete;
-const unique $StringConst1 : ref extends  complete;
-const unique $StringConst2 : ref extends  complete;
+const { :sourceloc "String.java",-1,-1,-1,-1 } unique java.lang.String : javaType extends  unique java.lang.Comparable, unique java.lang.CharSequence, unique java.lang.Object, unique java.io.Serializable complete;
+const { :sourceloc "InfeasibleCode02.java",-1,-1,-1,-1 } unique InfeasibleCode02 : javaType extends  unique java.lang.Object complete;
 var $heap : $heap_type;
 var $intArrayType : javaType;
 var $charArrayType : javaType;
@@ -30,7 +28,8 @@ var $boolArrHeap : boolArrHeap_type;
 var $refArrHeap : refArrHeap_type;
 var $realArrHeap : realArrHeap_type;
 var $intArrHeap : intArrHeap_type;
-var int$FalsePositives$countSource0 : Field int;
+var int$InfeasibleCode01$beginEndTag0 : Field int;
+var int$InfeasibleCode02$x0 : Field int;
 function $arrayType(t:javaType) returns ($ret:javaType);
 function $intToReal(x:int) returns ($ret:real);
 function $intToBool(x:int) returns ($ret:bool) { (if x == 0 then false else true) }
@@ -46,98 +45,257 @@ function $xorInt(x:int, y:int) returns ($ret:int);
 function $shlInt(x:int, y:int) returns ($ret:int);
 function $ushrInt(x:int, y:int) returns ($ret:int);
 function $shrInt(x:int, y:int) returns ($ret:int);
-procedure $new(obj_type:javaType) returns ($obj:ref);        requires $heap[$obj,$alloc] == false;    ensures $heap[$obj,$type] == obj_type;    ensures $heap[$obj,$alloc] == true;    ensures $obj != $null;
+procedure $new(obj_type:javaType) returns ($obj:ref);    ensures $obj != $null;    requires $heap[$obj,$alloc] == false;    ensures $heap[$obj,$type] == obj_type;    ensures $heap[$obj,$alloc] == true;    
 
-procedure java.lang.Object$java.lang.Object$clone$43($this:ref) returns ($other:ref);    ensures $heap[$other,$type] == $heap[$this,$type];    ensures $heap[$other,$alloc] == true;        ensures $other != $null;
+procedure java.lang.Object$java.lang.Object$clone$43($this:ref) returns ($other:ref);    ensures $other != $null;    ensures $heap[$other,$type] == $heap[$this,$type];        ensures $heap[$other,$alloc] == true;
 
-procedure int$java.lang.String$compareTo$87($this:ref, $other:ref) returns ($return:int);    ensures ($this == $other ==> $return == 1) && ($this != $other ==> $return == 0);    
+procedure int$java.lang.String$compareTo$87($this:ref, $other:ref) returns ($return:int);    
 
-procedure void$FalsePositives$FalsePositive02$1889($this:ref, $in_parameter__0:ref) returns ($exception:ref);    modifies $heap;
+procedure void$InfeasibleCode01$infeasible08$1889($this:ref, $in_parameter__0:ref, $in_parameter__1:ref, $in_parameter__2:int) returns ($exception:ref);    
 
-procedure java.lang.String$java.lang.Object$toString$44($this:ref) returns ($return:ref, $exception:ref);    
+procedure int$java.lang.String$indexOf$102($this:ref, $in_parameter__0:ref, $in_parameter__1:int) returns ($return:int, $exception:ref);    
 
-procedure void$FalsePositives$$la$init$ra$$1890($this:ref) returns ($exception:ref);    
+procedure void$InfeasibleCode01$$la$init$ra$$1890($this:ref) returns ($exception:ref);    
 
 procedure void$java.lang.Object$$la$init$ra$$38($this:ref) returns ($exception:ref);    
 
-implementation void$FalsePositives$FalsePositive02$1889($this:ref, $in_parameter__0:ref) returns ($exception:ref){
+procedure void$InfeasibleCode02$infeasible01$2084($this:ref) returns ($exception:ref);    
+
+procedure void$InfeasibleCode02$infeasible07$2085($this:ref, $in_parameter__0:ref) returns ($exception:ref);    
+
+procedure void$InfeasibleCode02$$la$init$ra$$2086($this:ref) returns ($exception:ref);    
+
+implementation void$InfeasibleCode01$infeasible08$1889($this:ref, $in_parameter__0:ref, $in_parameter__1:ref, $in_parameter__2:int) returns ($exception:ref){
     
-var temp$25 : int;    
-var temp$710 : int;    
-var htmlTag2 : ref;    
-var temp$36 : ref;    
-var temp$47 : int;    
-var temp$58 : int;    
-var temp$811 : int;    
-var temp$03 : ref;    
-var temp$69 : ref;    
-var this1 : ref;    
-var temp$14 : int;
+var searchString3 : ref;    
+var temp$412 : int;    
+var temp$513 : int;    
+var temp$311 : int;    
+var temp$614 : int;    
+var temp$816 : int;    
+var interncaret4 : int;    
+var source2 : ref;    
+var hitUp7 : int;    
+var flaghitup6 : int;    
+var temp$210 : int;    
+var temp$08 : int;    
+var temp$19 : int;    
+var temp$715 : int;    
+var temphitpoint5 : int;    
+var this1 : ref;
     assume $this != $null;
     this1 := $this;
-    htmlTag2 := $in_parameter__0;
-    assert { :sourceloc "FalsePositives.java",67,7,67,47 } htmlTag2 != $null;
-    call temp$03, $exception := java.lang.String$java.lang.Object$toString$44(htmlTag2);
-    assert { :sourceloc "FalsePositives.java",67,7,67,47 } temp$03 != $null;
-    call temp$14 := int$java.lang.String$compareTo$87(temp$03, $StringConst0);
-    if (temp$14 == 0) {
-        assert { :sourceloc "FalsePositives.java",67,7,67,47 } true;
-        goto block1;
-    } else {
-        assert { :sourceloc "FalsePositives.java",67,7,67,47 } true;
-    }
-    goto block2;
+    source2 := $in_parameter__0;
+    searchString3 := $in_parameter__1;
+    interncaret4 := $in_parameter__2;
+    temphitpoint5 := -1;
+    flaghitup6 := 0;
+    hitUp7 := 0;
   block1:
-    temp$25 := 1;
-    assert { :sourceloc "FalsePositives.java",69,4,69,14 } this1 != $null;
-    $heap := $heap[this1,int$FalsePositives$countSource0 := temp$25];
+    temp$08 := 0;
+    flaghitup6 := temp$08;
+    assert { :sourceloc "InfeasibleCode01.java",96,4,96,60 } source2 != $null;
+    call temp$19, $exception := int$java.lang.String$indexOf$102(source2, searchString3, interncaret4);
+    temphitpoint5 := temp$19;
+    if (temphitpoint5 > 0) {
+        assert { :sourceloc "InfeasibleCode01.java",97,7,97,22 } true;
+        goto block2;
+    } else {
+        assert { :sourceloc "InfeasibleCode01.java",97,7,97,22 } true;
+    }
     goto block3;
   block2:
-    assert { :sourceloc "FalsePositives.java",71,12,71,49 } htmlTag2 != $null;
-    call temp$36, $exception := java.lang.String$java.lang.Object$toString$44(htmlTag2);
-    assert { :sourceloc "FalsePositives.java",71,12,71,49 } temp$36 != $null;
-    call temp$47 := int$java.lang.String$compareTo$87(temp$36, $StringConst1);
-    if (temp$47 == 0) {
-        assert { :sourceloc "FalsePositives.java",71,12,71,49 } true;
+    assert { :sourceloc "InfeasibleCode01.java",97,42,97,52 } this1 != $null;
+    temp$210 := $heap[this1,int$InfeasibleCode01$beginEndTag0];
+    if (temphitpoint5 < temp$210) {
+        assert { :sourceloc "InfeasibleCode01.java",97,42,97,52 } true;
         goto block4;
     } else {
-        assert { :sourceloc "FalsePositives.java",71,12,71,49 } true;
+        assert { :sourceloc "InfeasibleCode01.java",97,42,97,52 } true;
     }
-    goto block5;
+    goto block3;
+    goto block4;
   block4:
-    temp$58 := 2;
-    assert { :sourceloc "FalsePositives.java",73,4,73,14 } this1 != $null;
-    $heap := $heap[this1,int$FalsePositives$countSource0 := temp$58];
-    goto block6;
-  block5:
-    assert { :sourceloc "FalsePositives.java",75,12,75,49 } htmlTag2 != $null;
-    call temp$69, $exception := java.lang.String$java.lang.Object$toString$44(htmlTag2);
-    assert { :sourceloc "FalsePositives.java",75,12,75,49 } temp$69 != $null;
-    call temp$710 := int$java.lang.String$compareTo$87(temp$69, $StringConst2);
-    if (temp$710 == 0) {
-        assert { :sourceloc "FalsePositives.java",75,12,75,49 } true;
-        goto block7;
-    } else {
-        assert { :sourceloc "FalsePositives.java",75,12,75,49 } true;
-    }
-    goto block8;
-  block7:
-    temp$811 := 3;
-    assert { :sourceloc "FalsePositives.java",77,4,77,14 } this1 != $null;
-    $heap := $heap[this1,int$FalsePositives$countSource0 := temp$811];
-  block8:
-  block6:
+    temp$311 := hitUp7;
+    temp$412 := temp$311 + 1;
+    hitUp7 := temp$412;
+    temp$513 := 1;
+    flaghitup6 := temp$513;
+    temp$614 := temphitpoint5;
+    temp$715 := $stringSizeHeap[searchString3];
+    temp$816 := temp$614 + temp$715;
+    interncaret4 := temp$816;
   block3:
+    if (flaghitup6 == 0) {
+        assert { :sourceloc "InfeasibleCode01.java",103,11,103,19 } true;
+        goto block5;
+    } else {
+        assert { :sourceloc "InfeasibleCode01.java",103,11,103,19 } true;
+    }
+    goto block1;
+  block5:
+    if (hitUp7 == 0) {
+        assert { :sourceloc "InfeasibleCode01.java",104,6,104,15 } true;
+        goto block6;
+    } else {
+        assert { :sourceloc "InfeasibleCode01.java",104,6,104,15 } true;
+    }
+    goto block7;
+  block6:
+  block7:
     return;
 }
 
 
-implementation void$FalsePositives$$la$init$ra$$1890($this:ref) returns ($exception:ref){
+implementation void$InfeasibleCode01$$la$init$ra$$1890($this:ref) returns ($exception:ref){
     
-var this12 : ref;
+var this17 : ref;
     assume $this != $null;
-    this12 := $this;
-    call $exception := void$java.lang.Object$$la$init$ra$$38(this12);
+    this17 := $this;
+    call $exception := void$java.lang.Object$$la$init$ra$$38(this17);
+    return;
+}
+
+
+implementation void$InfeasibleCode02$infeasible01$2084($this:ref) returns ($exception:ref){
+    
+var temp$122 : int;    
+var temp$223 : int;    
+var temp$324 : int;    
+var temp$425 : int;    
+var counter20 : int;    
+var hit19 : int;    
+var temp$021 : int;    
+var this18 : ref;
+    assume $this != $null;
+    this18 := $this;
+    hit19 := 0;
+    counter20 := 0;
+  block8:
+    temp$021 := 0;
+    hit19 := temp$021;
+    assert { :sourceloc "InfeasibleCode02.java",67,7,67,7 } this18 != $null;
+    temp$122 := $heap[this18,int$InfeasibleCode02$x0];
+    if (temp$122 == counter20) {
+        assert { :sourceloc "InfeasibleCode02.java",67,7,67,7 } true;
+        goto block9;
+    } else {
+        assert { :sourceloc "InfeasibleCode02.java",67,7,67,7 } true;
+    }
+    goto block10;
+  block9:
+    temp$223 := counter20;
+    temp$324 := temp$223 + 1;
+    counter20 := temp$324;
+    temp$425 := 1;
+    hit19 := temp$425;
+    if (counter20 > 10000) {
+        assert { :sourceloc "InfeasibleCode02.java",71,8,71,22 } true;
+        goto block11;
+    } else {
+        assert { :sourceloc "InfeasibleCode02.java",71,8,71,22 } true;
+    }
+    goto block12;
+  block11:
+    return;
+  block12:
+  block10:
+    if (hit19 == 0) {
+        assert { :sourceloc "InfeasibleCode02.java",76,11,76,13 } true;
+        goto block13;
+    } else {
+        assert { :sourceloc "InfeasibleCode02.java",76,11,76,13 } true;
+    }
+    goto block8;
+  block13:
+    return;
+}
+
+
+implementation void$InfeasibleCode02$infeasible07$2085($this:ref, $in_parameter__0:ref) returns ($exception:ref){
+    
+var temp$233 : ref;    
+var j30 : int;    
+var temp$738 : int;    
+var temp$637 : int;    
+var temp$334 : int;    
+var temp$031 : int;    
+var this26 : ref;    
+var temp$536 : int;    
+var temp$839 : int;    
+var end29 : int;    
+var temp27 : ref;    
+var temp$435 : int;    
+var repos28 : int;    
+var temp$940 : int;    
+var temp$132 : int;
+    assume $this != $null;
+    this26 := $this;
+    temp27 := $in_parameter__0;
+    repos28 := -1;
+    end29 := -1;
+    j30 := end29;
+  block14:
+    temp$031 := j30;
+    temp$132 := temp$031 + 1;
+    j30 := temp$132;
+    temp$233 := temp27;
+    temp$334 := j30;
+    assert { :sourceloc "InfeasibleCode02.java",85,7,85,18 } temp$334 < $arrSizeHeap[temp$233] && temp$334 >= 0;
+    temp$435 := $intArrHeap[temp$233][temp$334];
+    temp$536 := temp$435;
+    if (temp$536 == 97) {
+        assert { :sourceloc "InfeasibleCode02.java",85,7,85,18 } true;
+        goto block15;
+    } else {
+        assert { :sourceloc "InfeasibleCode02.java",85,7,85,18 } true;
+    }
+    goto block16;
+  block15:
+    temp$637 := j30 - end29;
+    temp$738 := temp$637 - 1;
+    repos28 := temp$738;
+  block16:
+    if (repos28 == -1) {
+        assert { :sourceloc "InfeasibleCode02.java",88,11,88,21 } true;
+        goto block17;
+    } else {
+        assert { :sourceloc "InfeasibleCode02.java",88,11,88,21 } true;
+    }
+    goto block18;
+  block17:
+    assert { :sourceloc "InfeasibleCode02.java",88,26,88,40 } temp27 != $null;
+    temp$839 := $arrSizeHeap[temp27];
+    if (j30 < temp$839) {
+        assert { :sourceloc "InfeasibleCode02.java",83,2,88,42 } true;
+        goto block14;
+    } else {
+        assert { :sourceloc "InfeasibleCode02.java",88,26,88,40 } true;
+    }
+    goto block18;
+    goto block14;
+  block18:
+    if (repos28 == -1) {
+        assert { :sourceloc "InfeasibleCode02.java",89,6,89,16 } true;
+        goto block19;
+    } else {
+        assert { :sourceloc "InfeasibleCode02.java",89,6,89,16 } true;
+    }
+    goto block20;
+  block19:
+    temp$940 := 0;
+    repos28 := temp$940;
+  block20:
+    return;
+}
+
+
+implementation void$InfeasibleCode02$$la$init$ra$$2086($this:ref) returns ($exception:ref){
+    
+var this41 : ref;
+    assume $this != $null;
+    this41 := $this;
+    call $exception := void$java.lang.Object$$la$init$ra$$38(this41);
     return;
 }
 
